LeanMqtt/Primitives/OptType/Proofs.lean
@@ -4,21 +4,21 @@ import LeanMqtt.Primitives.OptType.Basic
 namespace Mqtt
 open Mqtt
 
-theorem OptType.roundtrip {α : Type} [c : Codec α] (b : Bool) (v : OptType α b) {rest : List UInt8} :
+theorem OptType.roundtrip {α : Type} [c : Codec α] [LawfulCodec α] (b : Bool) (v : OptType α b) {rest : List UInt8} :
     (OptType.parser b).run (serialize b v ++ rest) = some (v, rest) := by
   match b, v with
   | true,  val =>
-    exact @Codec.roundtrip α c val rest
+    exact @LawfulCodec.roundtrip α c _ val rest
   | false, ()  =>
     rfl
 
-theorem OptType.reconstruct {α : Type} [c : Codec α]
+theorem OptType.reconstruct {α : Type} [c : Codec α] [LawfulCodec α]
     (b : Bool) {v : OptType α b} {input rest : List UInt8} :
     (OptType.parser b).run input = some (v, rest) → input = serialize b v ++ rest := by
   intro h
   match b, v, h with
   | true, val, h =>
-    exact @Codec.reconstruct α c val input rest h
+    exact @LawfulCodec.reconstruct α c _ val input rest h
   | false, (), h =>
     injection h with h_pair
     injection h_pair with _ _
